MoreList.v
@@ -1,0 +1,157 @@
+From Coq Require Import List SetoidList.
+Import ListNotations.
+
+Set Implicit Arguments.
+
+(** * Some complements on lists *)
+
+Definition option_bind {A B} o (f:A->option B) :=
+ match o with
+ | None => None
+ | Some a => f a
+ end.
+
+(** An hybrid of [map] and [filter] *)
+
+Fixpoint mapfilter {A B} (f:A->option B) l :=
+ match l with
+ | [] => []
+ | a::l => match f a with
+           | Some b => b::mapfilter f l
+           | None => mapfilter f l
+           end
+ end.
+
+Lemma mapfilter_app {A B} (f:A->option B) l l' :
+  mapfilter f (l++l') = mapfilter f l ++ mapfilter f l'.
+Proof.
+induction l; simpl; auto.
+destruct f; simpl; auto; f_equal; auto.
+Qed.
+
+Instance mapfilter_ext {A B} :
+ Proper ((eq ==> eq) ==> eq ==> eq) (@mapfilter A B).
+Proof.
+ intros f f' E l l' <-.
+ induction l; simpl; auto.
+ rewrite <- (E a); auto. destruct f; auto. f_equal; auto.
+Qed.
+
+Lemma map_as_mapfilter {A B} (f:A->B) l :
+ map f l = mapfilter (fun a => Some (f a)) l.
+Proof.
+induction l; simpl; f_equal; auto.
+Qed.
+
+Lemma filter_as_mapfilter {A} (f:A->bool) l :
+ filter f l = mapfilter (fun a => if f a then Some a else None) l.
+Proof.
+induction l; simpl; auto. destruct f; simpl; auto. f_equal; auto.
+Qed.
+
+Lemma mapfilter_comp {A B C}(f:A->option B)(g:B->option C) l :
+ mapfilter g (mapfilter f l) = mapfilter (fun a => option_bind (f a) g) l.
+Proof.
+induction l; simpl; auto.
+destruct f; simpl; auto. destruct g; simpl; auto. f_equal; auto.
+Qed.
+
+Lemma mapfilter_map {A B C} (f:A->B)(g:B->option C) l :
+ mapfilter g (map f l) = mapfilter (fun a => g (f a)) l.
+Proof.
+now rewrite map_as_mapfilter, mapfilter_comp.
+Qed.
+
+Lemma map_mapfilter {A B C} (f:A->option B)(g:B->C) l :
+ map g (mapfilter f l) = mapfilter (fun a => option_map g (f a)) l.
+Proof.
+rewrite map_as_mapfilter, mapfilter_comp. f_equiv.
+Qed.
+
+(** Properties of [List.filter] *)
+
+Lemma filter_app {A} (f:A->bool) l l' :
+  filter f (l++l') = filter f l ++ filter f l'.
+Proof.
+induction l; simpl; auto. destruct (f a); simpl; f_equal; auto.
+Qed.
+
+Lemma filter_map {A B} (f:A->B)(h:B->bool) l :
+  filter h (map f l) = map f (filter (fun x => h (f x)) l).
+Proof.
+induction l; simpl; auto. destruct (h (f a)); simpl; f_equal; auto.
+Qed.
+
+Instance filter_ext {A} : Proper ((eq==>eq)==>eq==>eq) (@filter A).
+Proof.
+intros f f' E l l' <-.
+induction l; simpl; auto. rewrite <- (E a); auto.
+destruct f; simpl; auto. f_equal; auto.
+Qed.
+
+(** [List.partition] via [List.filter] *)
+
+Lemma partition_filter {A} (f:A->bool) l :
+ partition f l = (filter f l, filter (fun a => negb (f a)) l).
+Proof.
+induction l; simpl; auto. rewrite IHl. now destruct f.
+Qed.
+
+(** More results about [List.forallb] and [List.existsb] *)
+
+Lemma forallb_map {A B} (f:A->B)(h:B->bool) l:
+ forallb h (map f l) = forallb (fun a => h (f a)) l.
+Proof.
+induction l; simpl; auto. destruct h; simpl; auto.
+Qed.
+
+Lemma existsb_map {A B} (f:A->B)(h:B->bool) l:
+ existsb h (map f l) = existsb (fun a => h (f a)) l.
+Proof.
+induction l; simpl; auto. destruct h; simpl; auto.
+Qed.
+
+Instance forallb_ext {A} : Proper ((eq==>eq)==>eq==>eq) (@forallb A).
+Proof.
+intros f f' E l l' <-.
+induction l; simpl; auto. rewrite <- (E a); auto.
+destruct f; simpl; auto.
+Qed.
+
+Instance existsb_ext {A} : Proper ((eq==>eq)==>eq==>eq) (@existsb A).
+Proof.
+intros f f' E l l' <-.
+induction l; simpl; auto. rewrite <- (E a); auto.
+destruct f; simpl; auto.
+Qed.
+
+
+(** [SetoidList.SortA_app] written via a [iff] *)
+
+Section MoreOnSortA.
+Context {A} eqA `{Equivalence A eqA}.
+Context ltA `{StrictOrder A ltA} `{!Proper (eqA==>eqA==>iff) ltA}.
+
+Lemma SortA_app (l1 l2 : list A) :
+ sort ltA (l1++l2) <->
+ sort ltA l1 /\ sort ltA l2 /\
+  forall a1 a2, In a1 l1 -> In a2 l2 -> ltA a1 a2.
+Proof.
+ split.
+ { induction l1 as [|a1 l1 IHl1].
+   - easy.
+   - simpl. inversion_clear 1 as [ | ? ? Hs Hhd ].
+     destruct (IHl1 Hs) as (H1 & H2 & H3); clear IHl1.
+     repeat split.
+     * constructor; auto.
+       destruct l1; simpl in *; auto; inversion_clear Hhd; auto.
+     * trivial.
+     * intros b1 b2 [->|Hb1] Hb2; eauto.
+       eapply SortA_InfA_InA with (eqA:=eqA)(l:=l1++l2); auto.
+       rewrite InA_app_iff. right. apply In_InA; auto with *. }
+ { intros (U & V & W); eapply SortA_app; eauto.
+   intros x y. rewrite !InA_alt.
+   intros (x' & -> & Hx) (y' & -> & Hy); auto. }
+Qed.
+
+End MoreOnSortA.
